Source/DafnyRuntime.Tests/dafny/test/sample.dfy
@@ -1,6 +1,0 @@
-
-newtype int32 = x: int | 0 <= x < 0x1_0000_0000
-
-method Main() {
-  var x: seq<int32> := [1, 2, 3];
-}
