Source/DafnyRuntime/DafnyRuntimeDafny/test/dafnyRuntimeTest.dfy
@@ -1,0 +1,24 @@
+
+include "../src/dafnyRuntime.dfy"
+
+abstract module DafnyRuntimeTests {
+
+    import Dafny
+
+    method {:test} HappyPath() {
+        Dafny.EnsureSizeTLimitAboveMinimum();
+        var a := Dafny.NativeArray.Make<int>(5);
+        for i := 0 to 5 
+            invariant a.Valid()
+        {
+            a.Update(i as Dafny.size_t, i);
+        }
+        var frozen := a.Freeze(a.Length());
+        var s := new Dafny.ArraySequence(frozen);
+        for i: Dafny.size_t := 0 to 5 
+            invariant a.Valid()
+        {
+            expect s.Select(i) == i;
+        }
+    }
+}
